fix constraints for TensorCore GEMM by respecting warp size

src/lib/poly/gemm/Kuiper.Poly.GEMM.TensorCore.fst
@@ -30,12 +30,10 @@ open Kuiper.Matrix.Tiling
 open Kuiper.Poly.GEMM.Copy
 open Kuiper.Poly.GEMM.Tiled.Common
 
-// FIXME this says that every thread will own a tile, when in fact
-//  every warp should be owning a tile collectively!!!
-let live_thread_tile
+let live_warp_tile
   (#et : Type0) {| scalar et |}
   // Since this is an slprop, I would like to not erase the nat.
-  // Unfortunately, when unfolding live_thread_tile, after passing
+  // Unfortunately, when unfolding live_warp_tile, after passing
   // a (reveal x) as argument, this leads to (reveal (hide (reveal x)))
   // which creates problems with type equalities.
   (#rows : erased nat)
@@ -47,10 +45,10 @@ let live_thread_tile
   (tm : nat{tm > 0 /\ tm /? bm})
   (tn : nat{tn > 0 /\ tn /? bn})
   (bid : natlt ((rows/bm) * (cols/bn)))
-  (tid : natlt (bm/tm * (bn/tn)))
+  (wid : natlt (bm/tm * (bn/tn)))
   : slprop
   =
-    live (thread_tile (block_tile gC bm bn bid) tm tn tid)
+    live (warp_tile (block_tile gC bm bn bid) tm tn wid)
 
 // TODO look again at why we cannot use nats here instead of sizet
 unfold
@@ -73,7 +71,7 @@ let kpre1
   (tk : szp{tk /? bk})
   (fA fB : perm)
   (bid : enatlt (rows/bm * (cols/bn)))
-  (tid : enatlt (bm/tm * (bn/tn)))
+  (tid : natlt (bm/tm*(bn/tn)*warp_size))
   : slprop
   =
   pure (SZ.fits (rows * shared)) **
@@ -82,9 +80,9 @@ let kpre1
   pure (valid_frag_et_dims et_ab FragB tm tn tk) **
   pure (valid_frag_et_dims et_c FragAcc tm tn tk) **
   pure (valid_frag_et_comb et_ab et_c) **
-  gA |-> Frac (fA /. (rows/tm * (cols/tn))) eA **
-  gB |-> Frac (fB /. (rows/tm * (cols/tn))) eB **
-  live_thread_tile gC bm bn tm tn bid tid
+  gA |-> Frac (fA /. (rows/tm * (cols/tn) * warp_size)) eA **
+  gB |-> Frac (fB /. (rows/tm * (cols/tn) * warp_size)) eB **
+  live_warp_tile gC bm bn tm tn bid (tid/warp_size)
 
 unfold
 let kpost1
@@ -105,12 +103,12 @@ let kpost1
   (tn : szp{tn /? bn})
   (fA fB : perm)
   (bid : enatlt (rows/bm * (cols/bn)))
-  (tid : enatlt (bm/tm * (bn/tn)))
+  (tid : natlt (bm/tm*(bn/tn)*warp_size))
   : slprop
   =
-  gA |-> Frac (fA /. (rows/tm * (cols/tn))) eA **
-  gB |-> Frac (fB /. (rows/tm * (cols/tn))) eB **
-  live_thread_tile gC bm bn tm tn bid tid
+  gA |-> Frac (fA /. (rows/tm * (cols/tn) * warp_size)) eA **
+  gB |-> Frac (fB /. (rows/tm * (cols/tn) * warp_size)) eB **
+  live_warp_tile gC bm bn tm tn bid (tid/warp_size)
 
 let barrier_p
   (#et : Type0)
@@ -181,13 +179,13 @@ let kpre
   (fA fB : perm)
   (sh : c_shmems (shmems_desc et_ab bm bn bk))
   (bid : natlt (rows/bm * (cols/bn)))
-  (tid : natlt (bm/tm * (bn/tn)))
+  (tid : natlt (bm/tm*(bn/tn)*warp_size))
   : slprop
   =
   kpre1 gA eA gB eB gC bm bn bk tm tn tk fA fB bid tid **
-  exists* (x : seq _). fst sh |-> Frac (1.0R /. (bm/tm * (bn/tn))) x **
-  exists* (x : seq _). fst (snd sh) |-> Frac (1.0R /. (bm/tm * (bn/tn))) x **
-  barrier_tok (R.row_major bm bk) (R.row_major bk bn) (fst sh) (fst (snd sh)) 0 (bm/tm * (bn/tn)) tid
+  exists* (x : seq _). fst sh |-> Frac (1.0R /. (bm/tm*(bn/tn)*warp_size)) x **
+  exists* (x : seq _). fst (snd sh) |-> Frac (1.0R /. (bm/tm*(bn/tn)*warp_size)) x **
+  barrier_tok (R.row_major bm bk) (R.row_major bk bn) (fst sh) (fst (snd sh)) 0 (bm/tm * (bn/tn) * warp_size) tid
 
 unfold
 let kpost
@@ -210,13 +208,13 @@ let kpost
   (fA fB : perm)
   (sh : c_shmems (shmems_desc et_ab bm bn bk))
   (bid : natlt (rows/bm * (cols/bn)))
-  (tid : natlt (bm/tm * (bn/tn)))
+  (tid : natlt (bm/tm*(bn/tn)*warp_size))
   : slprop
   =
-  kpost1 (* comb *) gA eA gB eB gC bm bn bk tm tn fA fB bid tid **
-  exists* (x : seq _). fst sh |-> Frac (1.0R /. (bm/tm * (bn/tn))) x **
-  exists* (x : seq _). fst (snd sh) |-> Frac (1.0R /. (bm/tm * (bn/tn))) x **
-  barrier_tok (R.row_major bm bk) (R.row_major bk bn) (fst sh) (fst (snd sh)) (2 * (shared/bk)) (bm/tm * (bn/tn)) tid
+  kpost1 gA eA gB eB gC bm bn bk tm tn fA fB bid tid **
+  exists* (x : seq _). fst sh |-> Frac (1.0R /. (bm/tm*(bn/tn)*warp_size)) x **
+  exists* (x : seq _). fst (snd sh) |-> Frac (1.0R /. (bm/tm*(bn/tn)*warp_size)) x **
+  barrier_tok (R.row_major bm bk) (R.row_major bk bn) (fst sh) (fst (snd sh)) (2 * (shared/bk)) (bm/tm*(bn/tn)*warp_size) tid
 
 
 inline_for_extraction noextract
@@ -287,6 +285,7 @@ fn subproducts_tc
   ()
 }
 
+instance concerete_sz_32 : concrete_sz 32 = { x = 32sz }
 inline_for_extraction noextract
 fn epilogue
   (#et : Type0) {| scalar et |}
@@ -307,42 +306,39 @@ fn epilogue
   (accumFrag : fragment et FragAcc tm tn tk FragLAcc)
   (gC : gpu_matrix et (R.row_major rows cols))
   (bid : szlt (rows/bm * (cols/bn)))
-  (tid : szlt (bm/tm * (bn/tn)))
+  (tid : szlt (bm/tm * (bn/tn) * warp_size))
   requires
     gpu **
-    live_thread_tile gC bm bn tm tn bid tid **
+    live_warp_tile gC bm bn tm tn bid (tid/warp_size) **
     (exists* vaccumFrag.
       accumFrag |-> vaccumFrag)
   ensures
     gpu **
-    live_thread_tile gC bm bn tm tn bid tid **
+    live_warp_tile gC bm bn tm tn bid (tid/warp_size) **
     (exists* vaccumFrag.
       accumFrag |-> vaccumFrag)
 {
-  unfold live_thread_tile gC bm bn tm tn bid tid;
+  unfold live_warp_tile;
 
   (* Only create a tile in gC and write the accumulator values. In this version the input from gC
      was added by loading the tile into the accumulator before any other computations *)
-  let t_tile = thread_tile (block_tile gC (SZ.v bm) (SZ.v bn) (SZ.v bid))
-    (SZ.v tm) (SZ.v tn) (SZ.v tid);
-  assert (rewrites_to t_tile (thread_tile (block_tile gC (SZ.v bm) (SZ.v bn) (SZ.v bid))
-    (SZ.v tm) (SZ.v tn) (SZ.v tid)));
+  let w_tile = warp_tile (block_tile gC (SZ.v bm) (SZ.v bn) (SZ.v bid))
+    (SZ.v tm) (SZ.v tn) (SZ.v tid / warp_size);
+  assert (rewrites_to w_tile (warp_tile (block_tile gC (SZ.v bm) (SZ.v bn) (SZ.v bid))
+    (SZ.v tm) (SZ.v tn) (SZ.v tid / warp_size)));
 
   // from looking at the type of mma_store, it is not clear that cols mut be concretizable
   // 1. know that strided_row_major needs concrete sizes
   // 2. search the code base for the appropriate instance and see which of the arguments
   //   must be concretizable
   // 3. figure out which expression is which argument and make concretizable accordingly
-  mma_store accumFrag t_tile;
+  mma_store accumFrag w_tile;
 
-  // rewrite each t_tile as thread_tile (block_tile gC bm bn bid) tm tn tid;
-  fold live_thread_tile gC bm bn tm tn bid tid;
+  // rewrite each w_tile as warp_tile (block_tile gC bm bn bid) tm tn tid;
+  fold live_warp_tile;
   ()
 }
 
-// #push-options "--split_queries always --debug SMTFail"
-// #push-options "--z3rlimit 40 --retry 5"
-// #push-options "--print_implicits"
 inline_for_extraction noextract
 fn kf
   (#et_ab #et_c : Type0)
@@ -362,22 +358,22 @@ fn kf
   (tm : szp{tm /? bm})
   (tn : szp{tn /? bn})
   (tk : szp{tk /? bk})
-  (#_ : squash (SZ.fits (bm*bk + bm/tm*(bn/tn))))
-  (#_ : squash (SZ.fits (bk*bn + bm/tm*(bn/tn))))
+  (#_ : squash (SZ.fits (bm*bk + bm/tm*(bn/tn)*warp_size -1)))
+  (#_ : squash (SZ.fits (bk*bn + bm/tm*(bn/tn)*warp_size -1)))
   (#fA #fB : perm)
   (sh : c_shmems (shmems_desc et_ab bm bn bk))
   (bid : szlt (rows/bm * (cols/bn)))
-  (tid : szlt (bm/tm * (bn/tn)))
+  (tid : szlt (bm/tm * (bn/tn) * warp_size))
   ()
   requires
     gpu **
     kpre gA eA gB eB gC bm bn bk tm tn tk fA fB sh bid tid **
-    thread_id (bm/tm * (bn/tn)) tid **
+    thread_id (bm/tm * (bn/tn) * warp_size) tid **
     block_id (rows/bm * (cols/bn)) bid
   ensures
     gpu **
-    kpost (* comb *) gA eA gB eB gC bm bn bk tm tn fA fB sh bid tid **
-    thread_id (bm/tm * (bn/tn)) tid **
+    kpost gA eA gB eB gC bm bn bk tm tn fA fB sh bid tid **
+    thread_id (bm/tm * (bn/tn) * warp_size) tid **
     block_id (rows/bm * (cols/bn)) bid
 {
   let sarA : gpu_array et_ab (bm * bk) = fst sh;
@@ -392,7 +388,7 @@ fn kf
   // assert (rewrites_to slA (R.row_major bm bk));
   // let slB = R.row_major bk bn;
   // assert (rewrites_to slB (R.row_major bk bn));
-  unfold barrier_tok (R.row_major bm bk) (R.row_major bk bn) sarA sarB 0 (bm/tm * (bn/tn)) tid;
+  unfold barrier_tok (R.row_major bm bk) (R.row_major bk bn) sarA sarB 0 (bm/tm * (bn/tn) * warp_size) tid;
 
   gpu_matrix_abs' (R.row_major bm bk) sarA;
   let sA = from_array (R.row_major bm bk) sarA;
@@ -407,8 +403,9 @@ fn kf
   let mrow = bid /^ num_n_tiles;
   let mcol = bid %^ num_n_tiles;
 
-  let threadRow = tid /^ (bn/^tn);
-  let threadCol = tid %^ (bn/^tn);
+  let wid = tid /^ warp_sz;
+  let threadRow = wid /^ (bn/^tn);
+  let threadCol = wid %^ (bn/^tn);
 
   (* tensor core fragments *)
   let aFrag = __alloc_fragment et_ab FragA tm tn tk FragLRM;
@@ -416,11 +413,11 @@ fn kf
   let accumFrag = __alloc_fragment et_c FragAcc tm tn tk FragLAcc;
 
   (* get ownership over the thread's gC tile and load it into the accumulator *)
-  unfold live_thread_tile gC bm bn tm tn bid tid;
-  let t_tile = thread_tile (block_tile gC (SZ.v bm) (SZ.v bn) (SZ.v bid)) (SZ.v tm) (SZ.v tn) (SZ.v tid);
-  assert (rewrites_to t_tile (thread_tile (block_tile gC (SZ.v bm) (SZ.v bn) (SZ.v bid)) (SZ.v tm) (SZ.v tn) (SZ.v tid)));
+  unfold live_warp_tile;
+  let t_tile = warp_tile (block_tile gC (SZ.v bm) (SZ.v bn) (SZ.v bid)) (SZ.v tm) (SZ.v tn) (SZ.v tid / warp_size);
+  assert (rewrites_to t_tile (warp_tile (block_tile gC (SZ.v bm) (SZ.v bn) (SZ.v bid)) (SZ.v tm) (SZ.v tn) (SZ.v tid / warp_size)));
   mma_loadAccum accumFrag t_tile;
-  fold live_thread_tile gC bm bn tm tn bid tid;
+  fold live_warp_tile;
 
   let mut bkIdx  : sz = 0sz;
   while (SZ.(!bkIdx <^ num_k_tiles))
@@ -432,44 +429,45 @@ fn kf
         aFrag |-> vaFrag **
         bFrag |-> vbFrag **
         accumFrag |-> vaccumFrag **
-        (exists* (x : ematrix _ _ _). sA |-> Frac (1.0R /. ((bm/tm*(bn/tn)))) x) **
-        (exists* (x : ematrix _ _ _). sB |-> Frac (1.0R /. ((bm/tm*(bn/tn)))) x) **
-        B.barrier_tok (barrier_p sA sB ((bm/tm*(bn/tn)))) (barrier_q sA sB ((bm/tm*(bn/tn)))) (2 * !bkIdx) tid
+        (exists* (x : ematrix _ _ _). sA |-> Frac (1.0R /. ((bm/tm*(bn/tn) * warp_size))) x) **
+        (exists* (x : ematrix _ _ _). sB |-> Frac (1.0R /. ((bm/tm*(bn/tn) * warp_size))) x) **
+        B.barrier_tok (barrier_p sA sB ((bm/tm*(bn/tn)* warp_size))) (barrier_q sA sB ((bm/tm*(bn/tn) * warp_size))) (2 * !bkIdx) tid
   {
     (* This assert should not be needed. I don't know what effect it even has. *)
-    assert B.barrier_tok (barrier_p sA sB (bm/tm * (bn/tn))) (barrier_q sA sB (bm/tm * (bn/tn))) (2 * !bkIdx) tid;
+    assert B.barrier_tok (barrier_p sA sB (bm/tm * (bn/tn) * warp_size)) (barrier_q sA sB (bm/tm * (bn/tn) * warp_size)) (2 * !bkIdx) tid;
     even_2x !bkIdx;
     assert pure((2 * !bkIdx % 2 = 0) == true);
     // binding only required because of rewrite
+    // TODO Remove after merging newest FStar updates
     let vbkIdx = !bkIdx;
     rewrite
-        (exists* (x : ematrix _ _ _). sA |-> Frac (1.0R /. (bm/tm * (bn/tn))) x) **
-        (exists* (x : ematrix _ _ _). sB |-> Frac (1.0R /. (bm/tm * (bn/tn))) x)
-      as barrier_p sA sB (bm/tm * (bn/tn)) (2 * vbkIdx) tid;
+        (exists* (x : ematrix _ _ _). sA |-> Frac (1.0R /. (bm/tm * (bn/tn) * warp_size)) x) **
+        (exists* (x : ematrix _ _ _). sB |-> Frac (1.0R /. (bm/tm * (bn/tn) * warp_size)) x)
+      as barrier_p sA sB (bm/tm * (bn/tn) * warp_size) (2 * vbkIdx) tid;
 
     B.barrier_wait ();
-    rewrite (barrier_q sA sB (bm/tm * (bn/tn)) (2 * vbkIdx) tid)
-        as live_tile_stride_cells sA (bm/tm * (bn/tn)) tid **
-           live_tile_stride_cells sB (bm/tm * (bn/tn)) tid;
+    rewrite (barrier_q sA sB (bm/tm * (bn/tn) * warp_size) (2 * vbkIdx) tid)
+        as live_tile_stride_cells sA (bm/tm * (bn/tn) * warp_size) tid **
+           live_tile_stride_cells sB (bm/tm * (bn/tn) * warp_size) tid;
 
     populate_shmem bm bn bk tm tn sA sB gA gB mrow !bkIdx mcol tid;
 
-    assert (B.barrier_tok (barrier_p sA sB (bm/tm * (bn/tn))) (barrier_q sA sB (bm/tm * (bn/tn))) (2 * vbkIdx + 1) tid);
+    assert (B.barrier_tok (barrier_p sA sB (bm/tm * (bn/tn) * warp_size)) (barrier_q sA sB (bm/tm * (bn/tn) * warp_size)) (2 * vbkIdx + 1) tid);
     odd_2x1 vbkIdx;
     assert (pure (odd (2 * vbkIdx + 1)));
-    rewrite live_tile_stride_cells sA (bm/tm * (bn/tn)) tid **
-            live_tile_stride_cells sB (bm/tm * (bn/tn)) tid
-         as (barrier_p sA sB (bm/tm * (bn/tn)) (2 * vbkIdx + 1) tid);
+    rewrite live_tile_stride_cells sA (bm/tm * (bn/tn) * warp_size) tid **
+            live_tile_stride_cells sB (bm/tm * (bn/tn) * warp_size) tid
+         as (barrier_p sA sB (bm/tm * (bn/tn) * warp_size) (2 * vbkIdx + 1) tid);
 
     B.barrier_wait ();
 
     even_2x (vbkIdx + 1);
     assert (pure (2 * (vbkIdx + 1) == 2 * vbkIdx + 2));
     assert (pure (even (2 * vbkIdx + 2)));
-    rewrite (barrier_q sA sB (bm/tm * (bn/tn)) (2 * vbkIdx + 1) tid)
+    rewrite (barrier_q sA sB (bm/tm * (bn/tn) * warp_size) (2 * vbkIdx + 1) tid)
     as
-      (exists* (x : ematrix _ _ _). sA |-> Frac (1.0R /. (bm/tm * (bn/tn))) x) **
-      (exists* (x : ematrix _ _ _). sB |-> Frac (1.0R /. (bm/tm * (bn/tn))) x);
+      (exists* (x : ematrix _ _ _). sA |-> Frac (1.0R /. (bm/tm * (bn/tn) * warp_size)) x) **
+      (exists* (x : ematrix _ _ _). sB |-> Frac (1.0R /. (bm/tm * (bn/tn) * warp_size)) x);
 
     subproducts_tc bm bn bk tm tn tk aFrag bFrag accumFrag sA sB threadRow threadCol;
 
@@ -485,7 +483,7 @@ fn kf
   gpu_matrix_concr sA; rewrite each core sA as sarA;
   gpu_matrix_concr sB; rewrite each core sB as sarB;
 
-  fold barrier_tok (R.row_major bm bk) (R.row_major bk bn) sarA sarB (2 * num_k_tiles) (bm/tm * (bn/tn)) tid;
+  fold barrier_tok (R.row_major bm bk) (R.row_major bk bn) sarA sarB (2 * num_k_tiles) (bm/tm * (bn/tn) * warp_size) tid;
 
   rewrite each sarA as fst sh;
   rewrite each sarB as fst (snd sh);
@@ -517,7 +515,7 @@ fn setup
   (tn : szp{tn /? bn})
   (tk : szp{tk /? bk})
   (nblk : szp{SZ.v nblk == rows/bm * (cols/bn)})
-  (nthr : szp{SZ.v nthr == bm/tm * (bn/tn)})
+  (nthr : szp{SZ.v nthr == bm/tm * (bn/tn) * warp_size})
   (fA fB : perm)
   ()
   norewrite
@@ -559,7 +557,7 @@ fn block_setup
   (tn : szp{tn /? bn})
   (tk : szp{tk /? bk})
   (nblk : szp{SZ.v nblk == rows/bm * (cols/bn)})
-  (nthr : szp{SZ.v nthr == bm/tm * (bn/tn)})
+  (nthr : szp{SZ.v nthr == bm/tm * (bn/tn) * warp_size})
   (fA fB : perm)
   (sh : c_shmems (shmems_desc et_ab bm bn bk))
   (bid : natlt nblk)
@@ -602,7 +600,7 @@ fn block_teardown
   (tm : szp{tm /? bm})
   (tn : szp{tn /? bn})
   (nblk : szp{SZ.v nblk == rows/bm * (cols/bn)})
-  (nthr : szp{SZ.v nthr == bm/tm * (bn/tn)})
+  (nthr : szp{SZ.v nthr == bm/tm * (bn/tn) * warp_size})
   (fA fB : perm)
   (sh : c_shmems (shmems_desc et_ab bm bn bk))
   (bid : natlt nblk)
@@ -642,7 +640,7 @@ fn teardown
   (tm : szp{tm /? bm})
   (tn : szp{tn /? bn})
   (nblk : szp{SZ.v nblk == rows/bm * (cols/bn)})
-  (nthr : szp{SZ.v nthr == bm/tm * (bn/tn)})
+  (nthr : szp{SZ.v nthr == bm/tm * (bn/tn) * warp_size})
   (fA fB : perm)
   ()
   norewrite
@@ -691,76 +689,46 @@ let mk_kernel
   (tk : szp{tk /? bk})
   (#fA #fB : perm)
   (nblk : szp{SZ.v nblk == rows/bm * (cols/bn)})
-  (nthr : szp{SZ.v nthr == bm/tm * (bn/tn)})
-  (#_ : squash (SZ.fits (bm*bk + bm/tm*(bn/tn))))
-  (#_ : squash (SZ.fits (bk*bn + bm/tm*(bn/tn))))
-  (#_ : squash (rows/bm * (cols/bn) <= max_blocks
-               /\ (bm/tm * (bn/tn)) <= max_threads))
+  // WARNING the previous version was wrong, it was assuming that each
+  //  thread computes tm*tk results similar to 2D-Blocktiling.
+  // There is nothing that catches this.
+  // (nthr : szp{SZ.v nthr == bm/tm * (bn/tn)})
+  // correct: the amount of tensor core tiles in gC multiplied
+  //  by the warp size (each warp computes one tile)
+  (nthr : szp{SZ.v nthr == bm/tm*(bn/tn)*warp_size})
+  (#_ : squash (valid_frag_et_dims et_ab FragA tm tn tk))
+  (#_ : squash (valid_frag_et_dims et_ab FragB tm tn tk))
+  (#_ : squash (valid_frag_et_dims et_c FragAcc tm tn tk))
+  (#_ : squash (valid_frag_et_comb et_ab et_c))
+  (#_ : squash (SZ.fits (bm*bk + nthr)))
+  (#_ : squash (SZ.fits (bk*bn + nthr)))
+  (#_ : squash (nblk <= max_blocks))
+  (#_ : squash (nthr <= max_threads))
   ()
   : kernel_desc
       (gA |-> Frac fA eA ** gB |-> Frac fB eB ** gC |-> eC)
       (gA |-> Frac fA eA ** gB |-> Frac fB eB ** (exists* eC'. gC |-> eC'))
 = {
-  nblk;// = rows/^bm *^ (cols/^bn);
-  nthr;// = (bm /^ tm *^ (bn /^ tn));
+  nblk;
+  nthr;
 
   shmems_desc = shmems_desc et_ab bm bn bk;
 
   frame = emp;
-  block_pre  = (fun bid -> forall+ (tid : natlt nthr). kpre1  (* comb *) gA eA gB eB gC bm bn bk tm tn tk fA fB bid tid);
-  block_post = (fun bid -> forall+ (tid : natlt nthr). kpost1 (* comb *) gA eA gB eB gC bm bn bk tm tn fA fB bid tid);
+  block_pre  = (fun bid -> forall+ (tid : natlt nthr). kpre1  gA eA gB eB gC bm bn bk tm tn tk fA fB bid tid);
+  block_post = (fun bid -> forall+ (tid : natlt nthr). kpost1 gA eA gB eB gC bm bn bk tm tn fA fB bid tid);
 
-  setup      = setup    (* comb *) gA eA gB eB gC eC bm bn bk tm tn tk nblk nthr fA fB;
-  teardown   = teardown (* comb *) gA eA gB eB gC eC bm bn bk tm tn nblk nthr fA fB;
+  setup      = setup    gA eA gB eB gC eC bm bn bk tm tn tk nblk nthr fA fB;
+  teardown   = teardown gA eA gB eB gC eC bm bn bk tm tn nblk nthr fA fB;
 
   block_frame    = (fun _ar _bid -> emp);
-  block_setup    = block_setup (* comb *) gA eA gB eB gC eC bm bn bk tm tn tk nblk nthr fA fB;
-  block_teardown = block_teardown (* comb *) gA eA gB eB gC eC bm bn bk tm tn nblk nthr fA fB ;
+  block_setup    = block_setup gA eA gB eB gC eC bm bn bk tm tn tk nblk nthr fA fB;
+  block_teardown = block_teardown gA eA gB eB gC eC bm bn bk tm tn nblk nthr fA fB ;
 
-  kpre      = kpre  (* comb *) gA eA gB eB gC bm bn bk tm tn tk fA fB;
-  kpost     = kpost (* comb *) gA eA gB eB gC bm bn bk tm tn fA fB;
+  kpre      = kpre  gA eA gB eB gC bm bn bk tm tn tk fA fB;
+  kpost     = kpost gA eA gB eB gC bm bn bk tm tn fA fB;
 
-  f = kf (* comb *) gA #eA gB #eB gC bm bn bk tm tn tk #() #() #fA #fB;
-}
-
-inline_for_extraction noextract
-fn mmcomb_gpu
-  (#et_ab #et_c : Type0)
-  {| scalar et_ab, scalar et_c |}
-  (#rows #shared #cols : szp)
-  (#lA : mlayout rows shared)
-  (#lB : mlayout shared cols)
-  {| clayout lA, clayout lB |}
-  (gA : gpu_matrix et_ab lA)
-  (#eA : ematrix et_ab rows shared)
-  (gB : gpu_matrix et_ab lB)
-  (#eB : ematrix et_ab shared cols)
-  (gC : gpu_matrix et_c (R.row_major rows cols))
-  (#_ : squash (SZ.fits (rows * cols)))
-  (#eC : ematrix et_c rows cols)
-  (bm : szp{bm /? rows})
-  (bn : szp{bn /? cols})
-  (bk : szp{bk /? shared})
-  (tm : szp{tm /? bm})
-  (tn : szp{tn /? bn})
-  (tk : szp{tk /? bk})
-  (#_ : squash (SZ.fits (bm*bk + bm/tm*(bn/tn))))
-  (#_ : squash (SZ.fits (bk*bn + bm/tm*(bn/tn))))
-  (#_: squash (SZ.fits (bm * bk) /\ SZ.fits (bk * bn)))
-  (#fA #fB : perm)
-  norewrite
-  preserves
-    cpu **
-    gA |-> Frac fA eA **
-    gB |-> Frac fB eB
-  requires
-    pure (rows/bm * (cols/bn) <= max_blocks) **
-    pure (bm/tm * (bn/tn) <= max_threads) **
-    gC |-> eC
-  ensures
-    (exists* eC'. gC |-> eC')
-{
-  launch_sync (mk_kernel gA gB gC bm bn bk tm tn tk (rows/^bm *^ (cols/^bn)) (bm/^tm *^ (bn/^tn)) ());
+  f = kf gA #eA gB #eB gC bm bn bk tm tn tk #() #() #fA #fB;
 }
 
 fn test
@@ -793,6 +761,6 @@ fn test
       #_ #(Kuiper.Matrix.Reprs.crepr_row_major.map _ _) gA #_
       #_ #(Kuiper.Matrix.Reprs.crepr_row_major.map _ _) gB #_
       gC
-      32sz 32sz 32sz 16sz 16sz 16sz (1024sz/^32sz *^ (1024sz/^32sz)) (32sz/^16sz *^ (32sz/^16sz)) ()
+      32sz 32sz 32sz 16sz 16sz 16sz (1024sz/^32sz *^ (1024sz/^32sz)) (32sz/^16sz *^ (32sz/^16sz) *^ warp_sz) ()
   );
 }
